pulse/pulse2rust/src/Pulse2Rust.Rust.Syntax.fst
@@ -21,6 +21,9 @@ let mk_vec_typ (t:typ) : typ =
     { typ_path_segment_name = "Vec"; typ_path_segment_generic_args = [t] };
   ]
 
+let mk_array_typ (t:typ) (len:expr) : typ =
+  Typ_array { typ_array_elem = t; typ_array_len = len }
+
 let mk_binop (l:expr) (op:binop) (r:expr) : expr =
   Expr_binop { expr_bin_left = l; expr_bin_op = op; expr_bin_right = r }
 
@@ -51,6 +54,9 @@ let mk_if (expr_if_cond:expr) (expr_if_then:list stmt) (expr_if_else:option expr
 
 let mk_while (expr_while_cond:expr) (expr_while_body:list stmt) : expr =
   Expr_while { expr_while_cond; expr_while_body }
+
+let mk_repeat (expr_repeat_elem expr_repeat_len:expr) : expr =
+  Expr_repeat { expr_repeat_elem; expr_repeat_len }
 
 let mk_scalar_fn_arg (name:string) (t:typ) =
   Fn_arg_pat {
